iris/SpecForkretParkPaid.v
@@ -262,7 +262,7 @@ Definition forkret_park_paid_body
     proc_priv γf pa pid V -∗
     fd_slots FDSPARE -∗
     iref_slots IREFSPARE -∗
-    |==> own_context cur_ctx ∗ ▷ proc_ctx γs pa.
+    |==> own_context cur_ctx ∗ proc_ctx_boxed γs pa.
 
 Module Type FORKRET_PARK_PAID.
   (* the residue is the module-type parameter it is everywhere else *)
